move continuity proofs to Coinductive

thys/Coinductive/Coinductive_List.thy
@@ -707,6 +707,12 @@ by(rule llist_partial_function_definitions)(simp)
 
 abbreviation "mono_llist \<equiv> monotone (fun_ord op \<sqsubseteq>) op \<sqsubseteq>"
 
+interpretation llist_lift!: partial_function_definitions "fun_ord lprefix" "fun_lub lSup"
+  where "fun_lub lSup {} \<equiv> \<lambda>_. LNil"
+by(rule llist_partial_function_definitions[THEN partial_function_lift])(simp)
+
+abbreviation "mono_llist_lift \<equiv> monotone (fun_ord (fun_ord lprefix)) (fun_ord lprefix)"
+
 lemma lprefixes_chain:
   "Complete_Partial_Order.chain op \<sqsubseteq> {ys. lprefix ys xs}"
 by(rule chainI)(auto dest: lprefix_down_linear)
@@ -1585,11 +1591,44 @@ by(simp_all add: ldrop.simps split: co.enat.split)
 lemma ldrop_lnull: "lnull xs \<Longrightarrow> ldrop n xs = LNil"
 by(simp add: lnull_def)
 
+lemma fixes f F
+  defines "F \<equiv> \<lambda>ldropn xs. case xs of LNil \<Rightarrow> \<lambda>_. LNil | LCons x xs \<Rightarrow> \<lambda>n. if n = 0 then LCons x xs else ldropn xs (n - 1)"
+  shows ldrop_conv_fixp: "(\<lambda>xs n. ldropn n xs) \<equiv> ccpo.fixp (fun_lub (fun_lub lSup)) (fun_ord (fun_ord lprefix)) (\<lambda>ldrop. F ldrop)" (is "?lhs \<equiv> ?rhs")
+  and ldrop_mono: "\<And>xs. mono_llist_lift (\<lambda>ldrop. F ldrop xs)" (is "PROP ?mono")
+proof(intro eq_reflection ext)
+  show mono: "PROP ?mono" unfolding F_def by(tactic {* Partial_Function.mono_tac @{context} 1 *})
+  fix n xs
+  show "?lhs xs n = ?rhs xs n"
+    by(induction n arbitrary: xs)
+      (subst llist_lift.mono_body_fixp[OF mono], simp add: F_def split: llist.split)+
+qed
+
+lemma ldropn_fixp_case_conv: 
+  "(\<lambda>xs. case xs of LNil \<Rightarrow> \<lambda>_. LNil | LCons x xs \<Rightarrow> \<lambda>n. if n = 0 then LCons x xs else f xs (n - 1)) =
+   (\<lambda>xs n. case xs of LNil \<Rightarrow> LNil | LCons x xs \<Rightarrow> if n = 0 then LCons x xs else f xs (n - 1))"
+by(auto simp add: fun_eq_iff split: llist.split)
+
+lemma monotone_ldropn_aux: "monotone lprefix (fun_ord lprefix) (\<lambda>xs n. ldropn n xs)"
+by(rule llist_lift.fixp_preserves_mono1[OF ldrop_mono ldrop_conv_fixp])
+  (simp add: ldropn_fixp_case_conv monotone_fun_ord_apply)
+
+lemma mono2mono_ldropn[THEN llist.mono2mono, cont_intro, simp]:
+  shows monotone_ldropn': "monotone lprefix lprefix (\<lambda>xs. ldropn n xs)"
+using monotone_ldropn_aux by(auto simp add: monotone_def fun_ord_def)
+
+lemma mcont_ldropn_aux: "mcont lSup lprefix (fun_lub lSup) (fun_ord lprefix) (\<lambda>xs n. ldropn n xs)"
+by(rule llist_lift.fixp_preserves_mcont1[OF ldrop_mono ldrop_conv_fixp])
+  (simp add: ldropn_fixp_case_conv mcont_fun_lub_apply)
+
+lemma mcont2mcont_ldropn [THEN llist.mcont2mcont, cont_intro, simp]:
+  shows mcont_ldropn: "mcont lSup lprefix lSup lprefix (ldropn n)"
+using mcont_ldropn_aux by(auto simp add: mcont_fun_lub_apply)
+
 lemma monotone_enat_cocase [cont_intro, simp]:
-  assumes mono: "\<And>n. monotone op \<le> ord (\<lambda>n. f n (eSuc n))"
-  and a: "\<And>n. ord a (f n (eSuc n))" "ord a a"
-  shows "monotone op \<le> ord (\<lambda>n. case n of 0 \<Rightarrow> a | eSuc n' \<Rightarrow> f n' n)"
-by(rule lfp.monotone_if_bot[where bot=a and bound=0 and f="\<lambda>n. f (epred n) n"])(auto simp add: neq_zero_conv_eSuc eSuc_le_iff monotoneD[OF mono] a)
+  "\<lbrakk> \<And>n. monotone op \<le> ord (\<lambda>n. f n (eSuc n));
+    \<And>n. ord a (f n (eSuc n)); ord a a \<rbrakk>
+  \<Longrightarrow> monotone op \<le> ord (\<lambda>n. case n of 0 \<Rightarrow> a | eSuc n' \<Rightarrow> f n' n)"
+by(rule monotone_enat_le_case)
 
 lemma monotone_ldrop: "monotone (rel_prod op = op \<sqsubseteq>) op \<sqsubseteq> (split ldrop)"
 by(rule llist.fixp_preserves_mono2[OF ldrop.mono ldrop_def]) simp
@@ -2624,6 +2663,32 @@ lemma ldropWhile_simps [simp, code]:
   shows ldropWhile_LNil: "ldropWhile P LNil = LNil"
   and ldropWhile_LCons: "ldropWhile P (LCons x xs) = (if P x then ldropWhile P xs else LCons x xs)"
 by(simp_all add: ldropWhile.simps)
+
+lemma fixes f F P
+  defines "F \<equiv> \<lambda>ltakeWhile xs. case xs of LNil \<Rightarrow> LNil | LCons x xs \<Rightarrow> if P x then LCons x (ltakeWhile xs) else LNil"
+  shows ltakeWhile_conv_fixp: "ltakeWhile P \<equiv> ccpo.fixp (fun_lub lSup) (fun_ord lprefix) F" (is "?lhs \<equiv> ?rhs")
+  and ltakeWhile_mono: "\<And>xs. mono_llist (\<lambda>ltakeWhile. F ltakeWhile xs)" (is "PROP ?mono")
+proof(intro eq_reflection ext)
+  show mono: "PROP ?mono" unfolding F_def by(tactic {* Partial_Function.mono_tac @{context} 1 *})
+  fix xs
+  show "?lhs xs = ?rhs xs"
+  proof(coinduction arbitrary: xs)
+    case Eq_llist
+    show ?case by(subst (1 3 4) llist.mono_body_fixp[OF mono])(auto simp add: F_def split: llist.split prod.split co.enat.split)
+  qed
+qed
+
+lemma mono2mono_ltakeWhile[THEN llist.mono2mono, cont_intro, simp]:
+  shows monotone_ltakeWhile: "monotone lprefix lprefix (ltakeWhile P)"
+by(rule llist.fixp_preserves_mono1[OF ltakeWhile_mono ltakeWhile_conv_fixp]) simp
+
+lemma mcont2mcont_ltakeWhile [THEN llist.mcont2mcont, cont_intro, simp]:
+  shows mcont_ltakeWhile: "mcont lSup lprefix lSup lprefix (ltakeWhile P)"
+by(rule llist.fixp_preserves_mcont1[OF ltakeWhile_mono ltakeWhile_conv_fixp]) simp
+
+lemma mono_llist_ltakeWhile [partial_function_mono]:
+  "mono_llist F \<Longrightarrow> mono_llist (\<lambda>f. ltakeWhile P (F f))"
+by(rule mono2mono_ltakeWhile)
 
 lemma mono2mono_ldropWhile [THEN llist.mono2mono, cont_intro, simp]:
   shows monotone_ldropWhile: "monotone op \<sqsubseteq> op \<sqsubseteq> (ldropWhile P)"
